mark-and-sweep/spec/GC.Spec.ChunkedSweepCoalesce.Compat.fsti
@@ -1,6 +1,7 @@
 module GC.Spec.ChunkedSweepCoalesce.Compat
 
 module U64 = FStar.UInt64
+module Seq = FStar.Seq
 
 open GC.Spec.Base
 open GC.Spec.Heap
@@ -8,6 +9,7 @@ open GC.Spec.Heap
 module Header = GC.Lib.Header
 module MH = GC.Spec.MajorHeap
 module Obj = GC.Spec.Object
+module Fields = GC.Spec.Fields
 module Defs = GC.Spec.ChunkedSweepCoalesce.Defs
 module SpecSweep = GC.Spec.Sweep
 
@@ -32,4 +34,24 @@ val chunked_sweep_object_single_chunk_compat
   : Lemma
       (Defs.chunked_sweep_object (MH.single_chunk_major_heap g) obj fp ==
        (let (g', fp') = SpecSweep.sweep_object g obj fp in
+        (MH.single_chunk_major_heap g', fp')))
+
+val chunked_sweep_aux_single_chunk_compat
+  (g: heap)
+  (objs: Seq.seq obj_addr)
+  (fp: U64.t)
+  : Lemma
+      (requires
+        (forall (o: obj_addr). Seq.mem o objs ==> U64.v o >= U64.v zero_addr + U64.v mword))
+      (ensures
+        Defs.chunked_sweep_aux (MH.single_chunk_major_heap g) objs fp ==
+        (let (g', fp') = SpecSweep.sweep_aux g objs fp in
+         (MH.single_chunk_major_heap g', fp')))
+
+val chunked_sweep_single_chunk_compat
+  (g: heap)
+  (fp: U64.t)
+  : Lemma
+      (Defs.chunked_sweep (MH.single_chunk_major_heap g) fp ==
+       (let (g', fp') = SpecSweep.sweep g fp in
         (MH.single_chunk_major_heap g', fp')))
